theories/Compositional_Structures/Basic_Modules/Component_Types/Electoral_Module_Ref.thy
@@ -18,34 +18,87 @@ definition em_rel :: "('a Electoral_Module_Ref \<times> 'a Electoral_Module) set
   "em_rel \<equiv> {(emref,em).(emref, (\<lambda> A pro. SPEC (\<lambda> res. res = (em A pro)))) 
   \<in> elec_mod_relb}"
 
+abbreviation "ballot_impl_assn \<equiv> (arl_assn nat_assn)"
 
-definition elect_ref ::
-  "'a Result \<Rightarrow> 'a set nres" where
-  "elect_ref result \<equiv> do {
-    RETURN (elect_r (result))}
-  "
-
-abbreviation "profile_impl_assn \<equiv> (list_assn (arl_assn nat_assn))"
+abbreviation "profile_impl_assn \<equiv> (list_assn ballot_impl_assn)"
 
 abbreviation "alts_set_impl_assn \<equiv> (hs.assn nat_assn)"
 
 abbreviation "result_impl_assn \<equiv> alts_set_impl_assn \<times>\<^sub>a alts_set_impl_assn \<times>\<^sub>a alts_set_impl_assn"
 
-definition "alts_assn \<equiv> hr_comp (hs.assn nat_assn) (\<langle>nat_rel\<rangle>alt_set_rel)"
+definition "alts_assn \<equiv> hr_comp alts_set_impl_assn (\<langle>nat_rel\<rangle>alt_set_rel)"
 
-definition "profile_assn \<equiv> (list_assn (hr_comp (list_assn nat_assn) ballot_rel))"
+definition "ballot_assn \<equiv> (hr_comp ballot_impl_assn ballot_rel)"
 
-abbreviation "result_assn \<equiv> hr_comp (hs.assn nat_assn) (\<langle>nat_rel\<rangle>set_rel) \<times>\<^sub>a
-                               hr_comp (hs.assn nat_assn) (\<langle>nat_rel\<rangle>set_rel) \<times>\<^sub>a
-                               hr_comp (hs.assn nat_assn) (\<langle>nat_rel\<rangle>set_rel)"
+definition "profile_assn \<equiv> (list_assn ballot_assn)"
+
+abbreviation "result_assn \<equiv> alts_assn \<times>\<^sub>a
+                              alts_assn \<times>\<^sub>a
+                               alts_assn"
 
 
-sepref_definition elect_sepref is 
-  "elect_ref" :: 
-   "(result_impl_assn)\<^sup>d \<rightarrow>\<^sub>a (hs.assn nat_assn)"
+locale sepref_access =
+  fixes mod1 :: "nat Electoral_Module_Ref"
+  fixes mod1_impl :: "(nat, unit) hashtable
+      \<Rightarrow> (nat array \<times> nat) list
+         \<Rightarrow> ((nat, unit) hashtable \<times> (nat, unit) hashtable \<times> (nat, unit) hashtable) Heap"
+  assumes 
+    mod1_impl: "(uncurry mod1_impl, uncurry mod1)
+        \<in> (alts_set_impl_assn)\<^sup>k *\<^sub>a profile_impl_assn\<^sup>k \<rightarrow>\<^sub>a result_impl_assn"
+
+begin
+
+  lemma this_loc: "sepref_access mod1 mod1_impl" by unfold_locales
+
+definition elect_ref ::
+  "nat set \<Rightarrow> nat Profile_List \<Rightarrow> nat set nres" where
+  "elect_ref A p \<equiv> do {
+    result <- mod1 A p;
+    RETURN (elect_r result)}
+  "
+
+lemma elect_monadic_refine:
+  fixes em:: "nat Electoral_Module"
+  assumes "(mod1,(\<lambda> A p. SPEC (\<lambda> rem. rem = em A p))) \<in> elec_mod_relb"
+  shows "(elect_ref, (\<lambda> A p. SPEC (\<lambda> rem. rem = (elect em A p)))) \<in> 
+    \<langle>nat_rel\<rangle>alt_set_rel \<rightarrow> profile_rel \<rightarrow> \<langle>\<langle>nat_rel\<rangle>alt_set_rel\<rangle>nres_rel"
   unfolding elect_ref_def
-  apply sepref_dbg_keep
-  done
+proof (refine_vcg, rename_tac A' A pl pr)
+   fix A' A:: "nat set"
+  fix pl :: "nat Profile_List"
+  fix pr :: "nat Profile"
+  assume arel: "(A', A) \<in> \<langle>nat_rel\<rangle>alt_set_rel"
+  assume prel: " (pl, pr) \<in> profile_rel"
+  from arel have aeq: "A' = A" by (auto simp add: alt_set_rel_def in_br_conv)
+  from arel have fina: "finite A'" by (auto simp add: alt_set_rel_def in_br_conv)
+  note assms[THEN fun_relD,THEN fun_relD, THEN nres_relD, where x2 = A' and x'2 = A
+      and x1 = pl and x'1 = pr]
+  from this have "  mod1 A' pl
+  \<le>  (SPEC (\<lambda>rem. rem = em A pr)) " using refine_IdD prod_rel_id set_rel_id
+    using arel prel by fastforce  
+  from this arel prel  show " mod1 A' pl \<bind> (\<lambda>result. RETURN (elect_r result))
+       \<le> \<Down> (\<langle>nat_rel\<rangle>alt_set_rel) (SPEC (\<lambda>rem. rem = elect em A pr))"
+    using specify_left
+    sorry
+qed
+  
 
+
+sepref_register "mod1" :: "nat Electoral_Module_Ref"
+
+declare mod1_impl [sepref_fr_rules]
+
+schematic_goal elect_impl:
+  "(uncurry ?c, uncurry elect_ref) \<in> (alts_set_impl_assn)\<^sup>k *\<^sub>a profile_impl_assn\<^sup>k \<rightarrow>\<^sub>a alts_set_impl_assn"
+  unfolding elect_ref_def
+  by sepref
+
+concrete_definition (in -) elect_sep uses sepref_access.elect_impl
+  prepare_code_thms (in -) elect_sep_def
+  lemmas elect_impl_refine = elect_sep.refine[OF this_loc]
+
+end
+
+term "sepref_access.elect_ref"
 
 end
